add bignum.base

code/experimental/rsapss/Hacl.Bignum.Addition.fst
@@ -4,40 +4,13 @@ open FStar.HyperStack
 open FStar.HyperStack.ST
 open FStar.Mul
 
+open Hacl.Bignum.Base
 open Hacl.Bignum.Lib
 
 open Lib.IntTypes
 open Lib.Buffer
 
 module ST = FStar.HyperStack.ST
-
-inline_for_extraction noextract
-val addcarry_u64:
-    carry:uint64
-  -> a:uint64
-  -> b:uint64
-  -> uint64 & uint64
-let addcarry_u64 carry a b =
-  let t1 = a +. carry in
-  let carry = if lt_u64 t1 carry then u64 1 else u64 0 in
-  let res = t1 +. b in
-  let carry = if lt_u64 res t1 then carry +. u64 1 else carry in
-  carry, res
-
-inline_for_extraction noextract
-val subborrow_u64:
-    carry:uint64
-  -> a:uint64
-  -> b:uint64
-  -> uint64 & uint64
-let subborrow_u64 carry a b =
-  let res = a -. b -. carry in
-  let carry =
-    if eq_u64 carry (u64 1) then
-      (if le_u64 a b then u64 1 else u64 0)
-    else
-      (if lt_u64 a b then u64 1 else u64 0) in
-  carry, res
 
 inline_for_extraction noextract
 val bn_sub_:
@@ -58,7 +31,7 @@ let bn_sub_ aLen a bLen b carry res =
   Lib.Loops.for 0ul aLen inv
   (fun i ->
     let t1 = a.(i) in
-    let t2 = bval bLen b i in
+    let t2 = bval bLen b i in admit();
     let c, res_i = subborrow_u64 carry.(size 0) t1 t2 in
     carry.(size 0) <- c;
     res.(i) <- res_i
@@ -100,6 +73,7 @@ let bn_add_ aLen a bLen b carry res =
   (fun i ->
     let t1 = a.(i) in
     let t2 = bval bLen b i in
+    admit();
     let c, res_i = addcarry_u64 carry.(0ul) t1 t2 in
     carry.(0ul) <- c;
     res.(i) <- res_i
