code/experimental/rsapss/Hacl.Bignum.Base.fst
@@ -1,0 +1,87 @@
+module Hacl.Bignum.Base
+
+open FStar.Mul
+open Lib.IntTypes
+
+#set-options "--z3rlimit 50 --max_fuel 0 --max_ifuel 0"
+
+inline_for_extraction noextract
+let carry = x:uint64{uint_v x == 0 \/ uint_v x == 1}
+
+inline_for_extraction noextract
+val eq_u64: a:uint64 -> b:uint64 -> Tot bool
+let eq_u64 a b =
+  let open Lib.RawIntTypes in
+  FStar.UInt64.(u64_to_UInt64 a =^ u64_to_UInt64 b)
+
+inline_for_extraction noextract
+val lt_u64: a:uint64 -> b:uint64 -> Tot bool
+let lt_u64 a b =
+  let open Lib.RawIntTypes in
+  FStar.UInt64.(u64_to_UInt64 a <^ u64_to_UInt64 b)
+
+inline_for_extraction noextract
+val le_u64: a:uint64 -> b:uint64 -> Tot bool
+let le_u64 a b =
+  let open Lib.RawIntTypes in
+  FStar.UInt64.(u64_to_UInt64 a <=^ u64_to_UInt64 b)
+
+
+inline_for_extraction noextract
+val addcarry_u64: c:carry -> a:uint64 -> b:uint64 ->
+  Pure (carry & uint64)
+  (requires True)
+  (ensures  fun (c', r) ->
+    uint_v r + uint_v c' * pow2 64 == uint_v a + uint_v b + uint_v c)
+
+let addcarry_u64 c a b =
+  let t1 = a +. c in
+  let c = if lt_u64 t1 c then u64 1 else u64 0 in
+  let res = t1 +. b in
+  let c = if lt_u64 res t1 then c +. u64 1 else c in
+  c, res
+
+
+inline_for_extraction noextract
+val subborrow_u64: c:carry -> a:uint64 -> b:uint64 ->
+  Pure (carry & uint64)
+  (requires True)
+  (ensures  fun (c', r) ->
+    uint_v r - uint_v c' * pow2 64 == uint_v a - uint_v b - uint_v c)
+
+let subborrow_u64 c a b =
+  let res = a -. b -. c in
+  let c =
+    if eq_u64 c (u64 1) then
+      (if le_u64 a b then u64 1 else u64 0)
+    else
+      (if lt_u64 a b then u64 1 else u64 0) in
+  c, res
+
+
+val lemma_mul_carry_add_64: a:uint64 -> b:uint64 -> c:uint64 -> d:uint64 ->
+  Lemma (uint_v a * uint_v b + uint_v c + uint_v d < pow2 128)
+let lemma_mul_carry_add_64 a b c d =
+  let n = pow2 64 in
+  assert (uint_v a <= n - 1 /\ uint_v b <= n - 1 /\ uint_v c <= n - 1 /\ uint_v d <= n - 1);
+  assert (uint_v a * uint_v b + uint_v c + uint_v d <= (n - 1) * (n - 1) + (n - 1) + (n - 1));
+  assert ((n - 1) * (n - 1) + (n - 1) + (n - 1) == n * n - 1);
+  FStar.Math.Lemmas.pow2_plus 64 64
+
+
+#set-options "--z3rlimit 100"
+
+inline_for_extraction noextract
+val mul_carry_add_u64: a:uint64 -> b:uint64 -> c:uint64 -> d:uint64 ->
+  Pure (tuple2 uint64 uint64)
+  (requires True)
+  (ensures  fun (c', r) ->
+    uint_v r + uint_v c' * pow2 64 == uint_v a * uint_v b + uint_v c + uint_v d)
+
+let mul_carry_add_u64 a b c d =
+  lemma_mul_carry_add_64 a b c d;
+  assert (uint_v a * uint_v b + uint_v c + uint_v d < pow2 128);
+  let res = mul64_wide a b +! to_u128 #U64 c +! to_u128 #U64 d in
+  let r = to_u64 res in
+  let c' = to_u64 (res >>. 64ul) in
+  c', r
